Defined decode_string_with_term and proved base case of half of the CorrectDecoder Theorem

src/Narcissus/Formats/WithTerm/String.v
@@ -1,12 +1,14 @@
 Require Import Coq.Strings.String.
 Require Import
+        Fiat.Narcissus.BinLib.AlignWord
         Fiat.Narcissus.Common.Notations
         Fiat.Narcissus.Common.Specs
         Fiat.Narcissus.Common.EquivFormat
         Fiat.Narcissus.Formats.Base.FMapFormat
         Fiat.Narcissus.Formats.Base.SequenceFormat
         Fiat.Narcissus.Formats.StringOpt
-        Fiat.Narcissus.Formats.Delimiter.
+        Fiat.Narcissus.Formats.Delimiter
+        Fiat.Narcissus.Formats.AsciiOpt.
 
 Section String.
   Context {B : Type}.
@@ -15,24 +17,155 @@ Section String.
   Context {monoid : Monoid B}.
   Context {monoidUnit : QueueMonoidOpt monoid bool}.
 
-  Definition decode_string_with_term (close : string)
-             (b : B) (cd : CacheDecode)
-    : option (string * B * CacheDecode).
-  Admitted.
+  Definition decode_string_with_term
+           (code: string)
+           (b : B) (cd : CacheDecode)
+    : option (string * B * CacheDecode) := 
+    (Fix well_founded_lt_b
+           (fun _ => CacheDecode -> option (string * B * CacheDecode))
+      (fun b rec cd =>
+     `(term_code, b', cd') <- decode_string (String.length code) b cd;
+      (* (peekD (T := string) cd) *)
+      If String.eqb code term_code Then
+        Some (EmptyString, b', cd')
+      Else
+        (`(a, b1, e1) <- Decode_w_Measure_lt decode_ascii b cd ltac:(exact ascii_decode_lt);
+        (`(xs, b2, e2) <- rec _ (proj2_sig b1) e1;
+        Some (String a xs, b2, e2)))) b cd).
+
+
+  Instance Equivalence_ S T : Equivalence (EquivFormat (S := S) (T := T)).
+  Proof.
+    constructor; 
+    red; 
+    [ apply EquivFormat_reflexive |
+      apply EquivFormat_sym |
+      apply EquivFormat_trans
+    ].
+  Qed.
+
+  Instance Symmetric_ S T : Symmetric (EquivFormat (S := S) (T := T)).
+  Proof.
+    red; auto.
+    intros.
+    symmetry.
+    auto.
+  Qed.
+
+  Add Parametric Morphism S T store M vP vP' decode P
+    : (fun format => CorrectDecoder (S := S)
+                    (T := T) (store := store) M vP vP' eq format decode P format) with
+        signature (@EquivFormat S T store) ==>
+                                           iff as cd_morph.
+  Proof using Type.
+    intros.
+    pose proof format_decode_correct_EquivFormatAndView_Proper.
+    do 2 red in H0.
+    simpl in H0.
+    unfold impl in H0.
+    split.
+    intros.
+    unfold flip in H0.
+    apply EquivFormat_sym in H.
+    eapply H0 in H; eauto.
+    intros.
+    eapply H0 in H; eauto.
+  Qed.
 
   Theorem string_decode_with_term_correct
           {P : CacheDecode -> Prop}
           (close : string)
-    : CorrectDecoder monoid
-                     (* TODO *)
-                     (fun s => True)
-                     (fun s => True)
-                     eq
-                     (format_with_term format_string close)
-                     (decode_string_with_term close)
-                     P
-                     (format_with_term format_string close).
+    : cache_inv_Property P
+    (fun P0 : CacheDecode -> Prop =>
+       forall (b : nat) (cd : CacheDecode), P0 cd -> P0 (addD cd b)) -> 
+    CorrectDecoder monoid
+                   (* This needs to be updated *)                                   
+                   (fun s => close <> "")%string
+                   (fun s => close <> "")%string
+                   eq
+                   (format_with_term format_string close)
+                   (decode_string_with_term close)
+                   P
+                   (format_with_term format_string close).
   Proof.
+    intros cach_inv.
+    split.
+    { intros env env' xenv s s' ext ? Eeq Ppred Penc.
+      generalize dependent env.
+      revert env' xenv s' env_OK.
+      induction s.
+      { unfold id in *; intros.
+        unfold format_with_term in Penc.
+        unfold "++" in Penc.
+        unfold compose in Penc.
+        simpl in Penc.
+        unfold Bind2 in Penc.
+        apply Bind_inv in Penc.
+        destruct_ex.
+        split_and.
+        apply Return_inv in H0.
+        rewrite <- H0 in H1.
+        simpl in H1.
+        apply Bind_inv in H1.
+        destruct H1.
+        destruct H.
+        rewrite mempty_left in H1.
+        apply Return_inv in H1.
+        inversion H1; subst.
+        clear H1.
+        pose proof H as Hsave.
+        unfold decode_string_with_term.
+        rewrite Init.Wf.Fix_eq.
+        destruct H.
+        split_and.
+        subst.
+        pose proof (String_decode_correct (P := P)).
+        destruct H with (sz := String.length x); eauto.
+        destruct x0.
+        eapply H1 in H0; eauto.
+        clear H H1 H2.
+        destruct_ex; split_and.
+        subst.
+        simpl.
+        rewrite H0.
+        simpl.
+        replace (x0 =? x0)%string with true by (auto using eqb_refl).
+        simpl.
+        exists ""%string, x1.
+        {
+          intuition; auto.
+          unfold format_with_term.
+          econstructor; eauto.
+          split.
+          unfold Ensembles.In.
+          simpl.
+          apply unfold_computes.
+          eapply ReturnComputes.
+          simpl.
+          red.
+          unfold Bind2.
+          apply unfold_computes.
+          eapply BindComputes; eauto.
+          rewrite mempty_left.
+          auto.
+        }
+        {
+          intros.
+          repeat (apply functional_extensionality; intros; f_equal).
+          subst; auto.
+          unfold DecodeBindOpt2.
+          unfold BindOpt.
+          unfold If_Opt_Then_Else.
+          destruct Decode_w_Measure_lt; auto.
+          do 2 destruct p; rewrite H0; auto.
+        }
+      }
+      {
+        admit.
+      }
+    }
+    {
+      admit.
+    }
   Admitted.
-
 End String.
